\documentclass[12pt]{extarticle}

\input{../preamble.tex}

\begin{document}

\subsection*{1.3}

% 1^3 + 2^3 ... + n^3 + (n+1)^3 = (1 + 2 + ... + n + (n+1))^2
% 1^3 + 2^3 ... + n^3 + (n+1)^3 = (1 + 2 + ... + n + (n+1))^2
% 1^3 + 2^3 ... + n^3 + (n+1)^3 = (1 + 2 + ... + n)^2 + 2(1 + 2 + ... + n)(n+1) + (n+1)^2
% 1^3 + 2^3 ... + n^3 + (n+1)^3 = (1 + 2 + ... + n)^2 + 2(1/2 (n (n+1)))(n+1) + (n+1)^2
% 1^3 + 2^3 ... + n^3 + (n+1)^3 = (1 + 2 + ... + n)^2 + n(n+1)(n+1) + (n+1)^2
% 1^3 + 2^3 ... + n^3 + (n+1)^3 = (1 + 2 + ... + n)^2 + n(n+1)^2 + (n+1)^2
% 1^3 + 2^3 ... + n^3 + (n+1)^3 = 1^3 + 2^3 ... + n^3 + (n+1)^3

\begin{proof}
	
\end{proof}

\subsection*{1.6}
%
% 11^n+1 - 4^n+1
% 11 * 11^n - 4 * 4^n
% 
%
\begin{proof}
	
\end{proof}

\end{document}
