\documentclass[12pt,titlepage]{extarticle}
\input{../preamble.tex}

\def\homeworknumber{1}
\input{hw_preamble.tex}

\begin{document}

% Section 2: #2
% Section 3: #1 (show your work)
% Section 6: #7, 10, 13
% Section 9: #5, 6, 8
% Section 11: #3, 5
% Section 12: #1, 4

\subsection*{2.2}
Let $z = x + iy$ such that $\Re(z) = x$ and $\Im(z) = y$.
\subsubsection*{Part A}

\[
    \Re(iz) = \Re(i(x + iy)) = \Re(ix - y) = \Re(- y + ix) = -y = -\Im(z)
.\]

\subsubsection*{Part B}
\[
    \Im(iz) = \Im(i(x + iy)) = \Im(- y + ix) = x = \Re(z)
.\]

\subsection*{3.1}
\subsubsection*{Part A}
\begin{align*}
    \frac{1+2i}{3-4i} + \frac{2-i}{5i} &=
    \frac{(1+2i)(\overline{3-4i})}{3^2 + (-4)^2} + \frac{(2-i)(\overline{5i})}{0^2 + 5^2} \\
    &= \frac{(1+2i)(3+4i)}{25} + \frac{(2-i)(-5i)}{25} \\
    &= \frac{3 + 4i + 6i + 8i^2}{25} + \frac{-10i + 5i^2}{25} \\
    &= \frac{-5 + 10i}{25} + \frac{-5 -10i}{25} \\
    &= -\frac{10}{25} = - \frac{2}{5}
\end{align*}

\subsubsection*{Part B}
\begin{align*}
    \frac{5i}{(1-i)(2-i)(3-i)} &= \frac{5i}{(2 - i - 2i + i^2)(3-i)} \\
    &= \frac{5i}{(1 - 3i)(3 - i)} \\
    &= \frac{5i}{3 - i - 9i + 3i^2} \\
    &= \frac{5i}{-10i} \\
    &= -\frac{5}{10} = -\frac{1}{2}
\end{align*}

\subsubsection*{Part C}
\[
    (1-i)^2 = 1 - 2i + i^2 = -2i \implies (1-i)^4 = (-2i)^2 = 4i^2 = -4
.\]

\subsection*{6.7}
\begin{align*}
    |\Re(2+\overline{z} + z^3)| &= \qty|\frac{2 + \overline{z} + z^3 + (\overline{2 + \overline{z} + z^3})}{2}| \\
    &= \qty|\frac{2 + \overline{z} + z^3 + 2 + z + \overline{z}^3}{2}| \\
    &= \qty|\frac{4 + z + \overline{z} + z^3 + 2}{2}| \\
    &\leq \frac{2 + |z| + |\overline{z}| + |z|^3 + |\overline{z}|^3}{2} \\
    &= \frac{2 + 2|z| + 2|z|^3}{2} \\
    &\leq \frac{2 + 2 + 2}{2} = 3 \leq 4
\end{align*}

\subsection*{6.10}
\begin{proof}
    Let $z = x + iy$.
    \begin{enumerate}
        \item[$\Rightarrow)$]
            Assume that $z$ is real. That is, $y = 0$. Then $z = x + 0y = x = x - 0y = \overline{z}$. Therefore $z = \overline{z}$
        \item[$\Leftarrow)$]
            Assume that $z = \overline{z}$. Then
            \[
                x + iy = x - iy
            .\]
            Equating the imaginary components gives $iy = - iy$ or equivalently $y = -y$. This is only true if $y = 0$. Therefore $z = x + 0y = x$ and hence $z$ is real.
    \end{enumerate}
    Both directions hence prove the if and only if.
\end{proof}

\subsection*{6.13}
\begin{align*}
    |z - z_0| = R \implies |z - z_0|^2 &= R^2 \\
    (z - z_0)\conj{(z - z_0)} &= R^2 \\
    (z - z_0) (\conj{z} - \conj{z_0}) &= R^2 \\
    z \conj{z} - z \conj{z_0} - \conj{z} z_0 + z_0 \conj{z_0} &= R^2 \\
    |z|^2 - z \conj{z_0} - \conj{z \conj{z_0}} + |z_0|^2 &= R^2 \\
    |z|^2 - (z \conj{z_0} + \conj{z \conj{z_0}}) + |z_0|^2 &= R^2 \\
    |z|^2 - 2 \Re(z \conj{z_0}) + |z_0|^2 &= R^2
\end{align*}

\subsection*{9.5}
\subsubsection*{Part A}
Since
\begin{align*}
    i &\Leftrightarrow e^{i\frac{\pi}{2}} \\
    1 - i\sqrt{3} &\Leftrightarrow 2e^{-i \frac{\pi}{3}} \\
    \sqrt{3} + i &\Leftrightarrow 2e^{i \frac{\pi}{6}}
\end{align*}
it follows that
\begin{align*}
    i (1 - i\sqrt{3})(\sqrt{3} + i) &= e^{i \frac{\pi}{2}} \cdot 2 e^{-i \frac{\pi}{3}} \cdot 2e^{i \frac{\pi}{6}} \\
    &= 4 e^{i\qty(\frac{\pi}{2} - \frac{\pi}{3} + \frac{\pi}{6})} \\
    &= 4e^{i \frac{\pi}{3}} \\
    &= 4 \cdot (\frac{1}{2} + i\frac{\sqrt{3}}{2}) = 2 \cdot (1 + i\sqrt{3})
\end{align*}

\subsubsection*{Part B}
Since
\begin{align*}
    5i &\Leftrightarrow 5 e^{i \frac{\pi}{2}} \\
    2 + i &\Leftrightarrow \sqrt{5} e^{i \arctan(\frac{1}{2})}
\end{align*}
Let $\theta = \arctan(\frac{1}{2})$. It follows
\begin{align*}
    \frac{5i}{2+i} &= 5e^{\pi \frac{\pi}{2}} \cdot \frac{1}{\sqrt{5}} e^{-i \theta} \\
                   &= \frac{5}{\sqrt{5}} e^{i \qty(\frac{\pi}{2} - \theta)} \\
                   &= \frac{5}{\sqrt{5}} (\cos(\frac{\pi}{2} - \theta) + i \sin(\frac{\pi}{2} - \theta)) \\
                   &= \frac{5}{\sqrt{5}} (\sin \theta - i \cos \theta) \\
                   &= \frac{5}{\sqrt{5}} (\sin \theta - i \cos \theta) \\
                   &= \frac{5}{\sqrt{5}} (\sin \theta - i \cos \theta) \\
\end{align*}

\subsubsection*{Part C}


\subsubsection*{Part D}

\subsection*{9.6}
\subsection*{9.8}

\subsection*{11.3}
\subsection*{11.5}

\subsection*{12.1}
\subsection*{12.4}


\end{document}
